WebAssembly/Wasm_Printing.thy
@@ -1,0 +1,11 @@
+theory Wasm_Printing imports Wasm_Checker_Printing Wasm_Interpreter_Printing Wasm_Type_Printing "HOL-Library.Code_Target_Nat" begin
+
+lemma [code]: "pred_option P None = True"
+  using Option.option.pred_inject(1)
+  by auto
+
+lemmas[code] = Option.option.pred_inject(2)
+
+export_code open typing run in OCaml file "code/Wasm_Executable.ml"
+
+end
